src/program_proof/wal/abstraction.v
@@ -1,12 +1,14 @@
 From RecordUpdate Require Import RecordSet.
 Import RecordSetNotations.
 
+From Goose.github_com.mit_pdos.goose_nfsd Require Import wal.
+
 From Perennial.program_proof Require Import proof_prelude.
 
 Module update.
   Record t :=
-    { addr: u64;
-      b: Block; }.
+    mk { addr: u64;
+         b: Block; }.
 End update.
 
 Definition disk := gmap Z Block.
@@ -23,3 +25,17 @@ Module log_state.
       }.
   Global Instance _eta: Settable _ := settable! mk <txn_disk; installed_to; durable_to>.
 End log_state.
+
+Section heap.
+Context `{!heapG Σ}.
+Definition update_val (up:u64*Slice.t): val :=
+  (#(fst up), slice_val (snd up))%V.
+
+Definition is_block (s:Slice.t) (b:Block) :=
+  is_slice_small s byteT (Block_to_vals b).
+
+Definition updates_slice (bk_s: Slice.t) (bs: list update.t): iProp Σ :=
+  ∃ bks, is_slice_small bk_s (struct.t Update.S) (update_val <$> bks) ∗
+   [∗ list] _ ↦ b_upd;upd ∈ bks;bs , let '(update.mk a b) := upd in
+                                     is_block (snd b_upd) b.
+End heap.
