src/program_proof/wal/circular_proof.v
@@ -1,0 +1,94 @@
+From Goose.github_com.mit_pdos.goose_nfsd Require Import wal.
+From Perennial.program_proof Require Import proof_prelude.
+From Perennial.program_proof Require Import wal.abstraction.
+
+Definition LogSz := 511.
+
+Section heap.
+Context `{!heapG Σ}.
+Context `{!crashG Σ}.
+Implicit Types (v:val).
+Implicit Types (stk:stuckness) (E:coPset).
+
+Implicit Types (upds: list update.t).
+
+Definition circ_data upds: iProp Σ :=
+  ⌜Z.of_nat (length upds) <= LogSz⌝ ∗
+  ∃ hdr1 hdr2, 0 d↦ hdr1 ∗ 1 d↦ hdr2 ∗ 2 d↦∗ (update.b <$> upds).
+
+(* TODO: write this abstraction relation *)
+Definition is_circular (l:loc) (upds: list update.t): iProp Σ :=
+  (∃ v, l ↦[struct.t circular.S] v) ∗ circ_data upds.
+
+Theorem is_circular_data_extract l upds :
+  is_circular l upds -∗ circ_data upds ∗ (circ_data upds -∗ is_circular l upds).
+Proof.
+  iIntros "[Hmem Hdata]".
+  iFrame.
+  iIntros "$".
+Qed.
+
+Theorem new_circular bs :
+  0 d↦∗ bs ∗ ⌜length bs = Z.to_nat (2+LogSz)⌝ -∗ ∃ upds, circ_data upds.
+Proof.
+Admitted.
+
+Theorem wp_recoverCircular upds :
+  {{{ circ_data upds }}}
+    recoverCircular #()
+  {{{ l, RET #l; is_circular l upds }}}.
+Proof.
+Admitted.
+
+Definition space_remaining upds: Z := LogSz - Z.of_nat (length upds).
+
+Theorem wp_circular__SpaceRemaining l upds :
+  {{{ is_circular l upds }}}
+    circular__SpaceRemaining #l
+  {{{ (x:u64), RET #x; ⌜int.val x = space_remaining upds⌝ ∗ is_circular l upds }}}.
+Proof.
+Admitted.
+
+Theorem wpc_circular__SpaceRemaining stk k E1 E2 l upds :
+  {{{ is_circular l upds }}}
+    circular__SpaceRemaining #l
+    @ stk; k; E1; E2
+  {{{ (x:u64), RET #x; ⌜int.val x = space_remaining upds⌝ ∗ is_circular l upds }}}
+  {{{ is_circular l upds }}}.
+Proof.
+Admitted.
+
+Theorem wpc_circular__appendFreeSpace stk k E1 E2 l upds bufs upds' :
+  0 < space_remaining upds ->
+  {{{ is_circular l upds ∗ updates_slice bufs upds' }}}
+    circular__appendFreeSpace #l (slice_val bufs)
+    @ stk; k; E1; E2
+                    (* TODO: need to break is_circular apart into the part
+                    consumed by the header and the free space; the free space
+                    gets modified here but not the in-memory state or existing
+                    updates *)
+  {{{ RET #(); is_circular l upds }}}
+  {{{ circ_data upds }}}.
+Proof.
+Admitted.
+
+Theorem wpc_circular__Append stk k E1 E2 l upds bufs upds' :
+  0 < space_remaining upds ->
+  {{{ is_circular l upds ∗ updates_slice bufs upds' }}}
+    circular__Append #l (slice_val bufs)
+    @ stk; k; E1; E2
+  {{{ RET #(); is_circular l (upds ++ upds') }}}
+  {{{ is_circular l upds ∨ is_circular l (upds ++ upds') }}}.
+Proof.
+Admitted.
+
+Theorem wpc_circular__Empty stk k E1 E2 l upds :
+  {{{ is_circular l upds }}}
+    circular__Empty #()
+    @ stk; k; E1; E2
+  {{{ RET #(); is_circular l [] }}}
+  {{{ circ_data upds ∨ circ_data [] }}}.
+Proof.
+Admitted.
+
+End heap.
